src/LamRefLogicFactsTotal_credits_perm.v
@@ -10,17 +10,18 @@ Require Import src.LambdaTotalTriple_credits_perm.
 Require Import src.Tactics.
 
 Require Import src.Interweave.
-Require Import src.Permutation.
 
 From Coq Require Import Lia.
 
 Ltac unfold_all :=
   unfold triple, hoare_triple, sa_exists, sa_forall, sa_credits, sa_star,
-    sa_single, sa_pure, sa_empty, sa_implies, disjoint_maps, labels.
+    sa_single_any, sa_single, sa_single_decl, sa_array_decl, sa_pure, sa_empty,
+    sa_implies, disjoint_maps, labels.
 
 Ltac unfold_all_in H :=
   unfold triple, hoare_triple, sa_exists, sa_forall, sa_credits, sa_star,
-    sa_single, sa_pure, sa_empty, sa_implies, disjoint_maps, labels in H.
+    sa_single_any, sa_single, sa_single_decl, sa_array_decl, sa_pure, sa_empty,
+    sa_implies, disjoint_maps, labels in H.
 
 Ltac subst_case_or :=
   match goal with
@@ -105,6 +106,31 @@ Lemma star_exists_l A (V : Set) (P : A -> StateAssertion V) Q c m :
   ((<exists> x, P x) <*> Q) c m <-> exists x, (P x <*> Q) c m.
 Proof.
   unfold_all. split; intros H; edestruct_direct; eauto 10.
+Qed.
+
+Lemma star_exists_l' V A P (Q : StateAssertion V) :
+  (<exists> x : A, P x) <*> Q ->> <exists> x : A, P x <*> Q.
+Proof.
+  unfold sa_implies. intros. apply star_exists_l. assumption.
+Qed.
+
+Lemma star_exists_r A (V : Set) P (Q : A -> StateAssertion V) c m :
+  (P <*> (<exists> x, Q x)) c m <-> exists x, (P <*> Q x) c m.
+Proof.
+  unfold_all; split; intros H; edestruct_direct; eauto 10.
+Qed.
+
+Lemma star_exists_r' V A (P : StateAssertion V) Q :
+  (P <*> (<exists> x : A, Q x)) ->> <exists> x : A, (P <*> Q x).
+Proof.
+  unfold sa_implies. intros. apply star_exists_r. assumption.
+Qed.
+
+Lemma exists_implies A (V : Set) (P Q : A -> StateAssertion V) :
+  (forall x, P x ->> Q x) ->
+  (<exists> x, P x) ->> (<exists> x, Q x).
+Proof.
+  unfold_all. intros. edestruct_direct.
 Qed.
 
 Ltac edestruct_all_in n :=
@@ -208,37 +234,6 @@ Proof.
     eauto 3 using star_implies_mono_valid.
 Qed.
 
-Theorem htriple_pure (V : Set) (e : Expr V) P Q :
-  (P -> hoare_triple e <[]> Q) <-> hoare_triple e <[P]> Q.
-Proof.
-  unfold hoare_triple, sa_pure, sa_empty.
-  split; intros; edestruct_direct.
-Qed.
-
-Theorem triple_pure (V : Set) (e : Expr V) P Q :
-  (P -> triple e <[]> Q) <-> triple e <[P]> Q.
-Proof.
-  unfold_all.
-  split; intros Htriple; intros; edestruct_direct; edestruct Htriple; eauto;
-    repeat eexists; eauto.
-Qed.
-
-Theorem htriple_exists A (V : Set) (e : Expr V) P Q :
-  (forall x : A, hoare_triple e (P x) Q) <->
-    hoare_triple e (<exists> x, P x) Q.
-Proof.
-  unfold hoare_triple, sa_exists.
-  split; intros; [edestruct_direct | edestruct_all].
-Qed.
-
-Theorem triple_exists A (V : Set) (e : Expr V) P Q :
-  (forall x : A, triple e (P x) Q) <-> triple e (<exists> x, P x) Q.
-Proof.
-  unfold_all.
-  split; intros Htriple; intros; edestruct_direct; edestruct Htriple; eauto;
-    repeat eexists; eauto.
-Qed.
-
 Theorem htriple_pure_post (V : Set) (e : Expr V) P Q :
   ((forall c m, Is_Valid_Map m -> P c m -> Q) /\
     hoare_triple e P (fun _ => <[]>)) <->
@@ -281,7 +276,7 @@ Lemma star_assoc_l (V : Set) (P : StateAssertion V) Q R :
   P <*> (Q <*> R) ->> (P <*> Q) <*> R.
 Proof.
   unfold_all. intros. edestruct_direct.
-  destruct Interweave_assoc_r with (Label * Value V)%type x0 x4 x6 x2 m as (?&?&?);
+  destruct Interweave_assoc_r with (Label * option (Value V))%type x0 x4 x6 x2 m as (?&?&?);
     auto.
   repeat eexists; eauto; intros.
   { apply map_Interweave with (f := fst) in H4, H5, H6, H7.
@@ -297,7 +292,7 @@ Lemma star_assoc_r (V : Set) (P : StateAssertion V) Q R :
   (P <*> Q) <*> R ->> P <*> (Q <*> R).
 Proof.
   unfold_all. intros. edestruct_direct.
-  destruct Interweave_assoc_l with (Label * Value V)%type x4 x6 x2 x0 m as (?&?&?);
+  destruct Interweave_assoc_l with (Label * option (Value V))%type x4 x6 x2 x0 m as (?&?&?);
     auto.
   repeat eexists; eauto; intros.
   { apply map_Interweave with (f := fst) in H3, H5, H6, H7.
@@ -340,6 +335,123 @@ Proof.
   apply Interweave_comm. assumption.
 Qed.
 
+Theorem htriple_pure (V : Set) (e : Expr V) P Q :
+  (P -> hoare_triple e <[]> Q) <-> hoare_triple e <[P]> Q.
+Proof.
+  unfold hoare_triple, sa_pure, sa_empty.
+  split; intros; edestruct_direct.
+Qed.
+
+Theorem triple_pure (V : Set) (e : Expr V) P Q :
+  (P -> triple e <[]> Q) <-> triple e <[P]> Q.
+Proof.
+  unfold_all.
+  split; intros Htriple; intros; edestruct_direct; edestruct Htriple; eauto;
+    repeat eexists; eauto.
+Qed.
+
+Theorem htriple_pure_star (V : Set) (e : Expr V) P H Q :
+  (P -> hoare_triple e H Q) <-> hoare_triple e (<[P]> <*> H) Q.
+Proof.
+  unfold hoare_triple, sa_pure, sa_star, sa_empty, disjoint_maps, labels.
+  split; intros; edestruct_direct;
+    try match goal with
+    | [p : ?P, H : ?P -> _ |- _] => specialize (H p)
+    end;
+    repeat invert_Intwv_nil; simpl in *; edestruct_all.
+  split_all; eauto. apply Interweave_nil_l.
+Qed.
+
+Theorem triple_pure_star (V : Set) (e : Expr V) P H Q :
+  (P -> triple e H Q) <-> triple e (<[P]> <*> H) Q.
+Proof.
+  unfold_all.
+  split; intros; edestruct_direct;
+    try match goal with
+    | [p : ?P, H : ?P -> _ |- _] => specialize (H p)
+    end;
+    repeat invert_Intwv_nil; simpl in *; edestruct_all;
+    split_all; eauto. apply Interweave_nil_l.
+Qed.
+
+Theorem htriple_exists A (V : Set) (e : Expr V) P Q :
+  (forall x : A, hoare_triple e (P x) Q) <->
+    hoare_triple e (<exists> x, P x) Q.
+Proof.
+  unfold hoare_triple, sa_exists.
+  split; intros; [edestruct_direct | edestruct_all].
+Qed.
+
+Theorem triple_exists A (V : Set) (e : Expr V) P Q :
+  (forall x : A, triple e (P x) Q) <-> triple e (<exists> x, P x) Q.
+Proof.
+  unfold_all.
+  split; intros Htriple; intros; edestruct_direct; edestruct Htriple; eauto;
+    repeat eexists; eauto.
+Qed.
+
+Theorem htriple_exists_star A (V : Set) (e : Expr V) H P Q :
+  (forall x : A, hoare_triple e (H <*> P x) Q) <->
+    hoare_triple e (H <*> <exists> x, P x) Q.
+Proof.
+  unfold hoare_triple, sa_star, sa_exists, disjoint_maps, labels.
+  split; intros; edestruct_direct; edestruct_all; split_all; eauto.
+Qed.
+
+Fact empty_spec (V : Set) c (m : Map V) :
+  <[]> c m <-> c = 0 /\ m = []%list.
+Proof.
+  unfold_all. reflexivity.
+Qed.
+
+Fact pure_spec (V : Set) P c (m : Map V) :
+  <[P]> c m <-> P /\ c = 0 /\ m = []%list.
+Proof.
+  unfold_all. reflexivity.
+Qed.
+
+Ltac normalize_star :=
+  repeat match goal with
+  | [H : <[]> ?c ?m |- _] => apply empty_spec in H as (?&?)
+  | [H : <[_]> ?c ?m |- _] => apply pure_spec in H as (?&?&?)
+  | [H : ((_ <*> _) <*> _) ?c ?m |- _] => apply star_assoc_r in H
+  | [H : (<[_]> <*> _) ?c ?m |- _] => apply star_pure_l in H as [? ?]
+  | [H : ((<exists> _, _) <*> _) ?c ?m |- _] => apply star_exists_l in H as [? ?]
+  | [H : (<exists> _, _) ?c ?m |- _] => destruct H
+  end.
+
+Ltac solve_star :=
+  repeat match goal with
+  | [H : <[]> ?c ?m |- _] => apply empty_spec; eauto
+  | [H : <[_]> ?c ?m |- _] => apply pure_spec; eauto
+  | [|- ((_ <*> _) <*> _) ?c ?m ] => apply star_assoc_l; eauto
+  | [|- (<[_]> <*> _) ?c ?m ] => apply star_pure_l; split; auto
+  | [|- ((<exists> _, _) <*> _) ?c ?m ] => apply star_exists_l; eexists; eauto
+  | [|- (<exists> _, _) ?c ?m] => eexists
+  end.
+
+Ltac swap_star :=
+  match goal with
+  | [|- (_ <*> _) ?c ?m] => apply star_comm
+  end.
+
+Ltac swap_star_ctx :=
+  match goal with
+  | [H : (_ <*> _) ?c ?m |- _] => apply star_comm in H
+  end.
+
+Theorem triple_exists_star A (V : Set) (e : Expr V) H P Q :
+  (forall x : A, triple e (H <*> P x) Q) <->
+    triple e (H <*> <exists> x, P x) Q.
+Proof.
+  unfold triple, hoare_triple.
+  split; intros.
+  - normalize_star. swap_star_ctx. normalize_star. swap_star_ctx.
+    normalize_star. swap_star_ctx. edestruct H0; eauto.
+  - edestruct H0; eauto. solve_star. swap_star. solve_star. swap_star.
+    solve_star. swap_star. eassumption.
+Qed.
+
 Lemma star_credits (V : Set) (k : nat) (P : StateAssertion V) c m :
   (sa_credits k <*> P) c m <->
     exists c', c = k + c' /\ P c' m.
@@ -347,6 +459,54 @@ Proof.
   unfold_all. split; intros; edestruct_direct.
   - invert_Intwv_nil. eauto.
   - split_all; eauto using Interweave_nil_l.
+Qed.
+
+Fact implies_trans (V : Set) (P Q R : StateAssertion V) :
+  P ->> Q ->
+  Q ->> R ->
+  P ->> R.
+Proof.
+  unfold_all. auto.
+Qed.
+
+Fact implies_spec (V : Set) (P Q : StateAssertion V) :
+  (P ->> Q) <-> forall c m, P c m -> Q c m.
+Proof.
+  unfold_all. reflexivity.
+Qed.
+
+Fact implies_post_spec (V : Set) (P Q : Value V -> StateAssertion V) :
+  (P -->> Q) <-> forall v c m, P v c m -> Q v c m.
+Proof.
+  unfold_all. reflexivity.
+Qed.
+
+Fact wand_star (V : Set) (P Q : StateAssertion V) :
+  ((P <-*> Q) <*> P) ->> Q.
+Proof.
+  unfold sa_wand, sa_implies. intros. normalize_star. swap_star_ctx. auto.
+Qed.
+
+Fact wand_star_r (V : Set) (P Q : StateAssertion V) :
+  (P <*> (P <-*> Q)) ->> Q.
+Proof.
+  eauto using star_comm, wand_star, implies_trans.
+Qed.
+
+Fact wand_wand (V : Set) (P Q R : StateAssertion V) :
+  (P <-*> Q) <*> (Q <-*> R) ->> (P <-*> R).
+Proof.
+  unfold sa_wand, sa_implies. intros. normalize_star. swap_star_ctx.
+  normalize_star. solve_star; eauto. intros ? ? H_sa.
+  eapply star_implies_mono in H_sa; [|apply implies_refl|apply star_comm].
+  apply star_assoc_l in H_sa.
+  eapply star_implies_mono in H_sa; eauto using implies_refl.
+Qed.
+
+Fact wand_wand_r (V : Set) (P Q R : StateAssertion V) :
+  (Q <-*> R) <*> (P <-*> Q) ->> (P <-*> R).
+Proof.
+  eauto using star_comm, wand_wand, implies_trans.
 Qed.
 
 Theorem triple_frame (V : Set) (e : Expr V) P Q H :
@@ -363,6 +523,287 @@ Theorem htriple_value (V : Set) (v : Value V) :
 Proof.
   unfold hoare_triple, sa_pure, sa_empty.
   intros m Hm. subst. eauto 10 with lamref.
+Qed.
+
+(** facts about StateAssertion *)
+
+Fact credits_star_l (V : Set) c1 c2 c :
+  c = c1 + c2 ->
+  sa_credits c1 <*> sa_credits c2 ->> sa_credits (V := V) c.
+Proof.
+  unfold_all. intros. edestruct_direct. invert_Intwv_nil. auto.
+Qed.
+
+Fact credits_star_r (V : Set) c1 c2 c :
+  c = c1 + c2 ->
+  sa_credits (V := V) c ->> sa_credits c1 <*> sa_credits c2.
+Proof.
+  unfold_all. intros. edestruct_direct. split_all; auto using Interweave_nil.
+Qed.
+
+Fact empty_star_l_intro (V : Set) (P : StateAssertion V) :
+  P ->> <[]> <*> P.
+Proof.
+  unfold_all. intros. split_all; eauto using Interweave_nil_l.
+Qed.
+
+Fact empty_star_r_intro (V : Set) (P : StateAssertion V) :
+  P ->> P <*> <[]>.
+Proof.
+  unfold_all. intros. split_all; eauto using Interweave_nil_r.
+Qed.
+
+Fact empty_star_l_cancel (V : Set) (P : StateAssertion V) :
+  <[]> <*> P ->> P.
+Proof.
+  unfold_all. intros. edestruct_direct. invert_Intwv_nil. auto.
+Qed.
+
+Fact empty_star_r_cancel (V : Set) (P : StateAssertion V) :
+  P <*> <[]> ->> P.
+Proof.
+  unfold_all. intros. edestruct_direct. rewrite Nat.add_0_r.
+  invert_Intwv_nil. auto.
+Qed.
+
+Fact disjoint_maps_nil_l V m :
+  @disjoint_maps V nil m.
+Proof.
+  unfold disjoint_maps. simpl. auto.
+Qed.
+
+Fact disjoint_maps_nil_r V m :
+  @disjoint_maps V m nil.
+Proof.
+  unfold disjoint_maps. simpl. auto.
+Qed.
+
+Fact equiv_sa_equiv V (P Q : StateAssertion V) :
+  P <<->> Q <-> forall c m, P c m <-> Q c m.
+Proof.
+  unfold sa_implies. split.
+  - intuition.
+  - intros Hequiv. split; intros; apply Hequiv; assumption.
+Qed.
+
+Lemma star_equiv_l V (P P' Q : StateAssertion V) :
+  P <<->> P' ->
+  (P <*> Q) <<->> (P' <*> Q).
+Proof.
+  repeat rewrite -> equiv_sa_equiv. intros Hequiv ? ?.
+  split; now (apply star_implies_mono; unfold sa_implies; intros;
+    [apply Hequiv|apply implies_refl]).
+Qed.
+
+Lemma star_equiv_r V (P Q Q' : StateAssertion V) :
+  Q <<->> Q' ->
+  (P <*> Q) <<->> (P <*> Q').
+Proof.
+  repeat rewrite -> equiv_sa_equiv. intros Hequiv ? ?.
+  split; now (apply star_implies_mono; unfold sa_implies; intros;
+    [apply implies_refl|apply Hequiv]).
+Qed.
+
+Lemma exists_equiv A P P' :
+  (forall x : A, P x <-> P' x) ->
+  (exists x, P x) <-> (exists x, P' x).
+Proof.
+  intros Hequiv. split; intros (?&?%Hequiv); eauto.
+Qed.
+
+Lemma sa_exists_equiv A V (P P' : A -> StateAssertion V) :
+  (forall x, P x <<->> P' x) ->
+  (<exists> x, P x) <<->> (<exists> x, P' x).
+Proof.
+  intros Hequiv. apply equiv_sa_equiv. intros. unfold sa_exists.
+  apply exists_equiv. intros. apply equiv_sa_equiv. auto.
+Qed.
+
+Lemma star_exists_equiv_l A V (P : A -> StateAssertion V) Q :
+  (<exists> x, P x) <*> Q <<->> (<exists> x, P x <*> Q).
+Proof.
+  rewrite equiv_sa_equiv. intros. apply star_exists_l.
+Qed.
+
+Lemma empty_star_l V (P : StateAssertion V) :
+  <[]> <*> P <<->> P.
+Proof.
+  apply equiv_sa_equiv. intros.
+  split; [apply empty_star_l_cancel|apply empty_star_l_intro].
+Qed.
+
+Lemma empty_star_r V (P : StateAssertion V) :
+  P <*> <[]> <<->> P.
+Proof.
+  apply equiv_sa_equiv. intros.
+  split; [apply empty_star_r_cancel|apply empty_star_r_intro].
+Qed.
+
+Fact sa_equiv_symm V (P Q : StateAssertion V) :
+  P <<->> Q ->
+  Q <<->> P.
+Proof.
+  repeat rewrite equiv_sa_equiv. intros. symmetry. eauto.
+Qed.
+
+Fact sa_equiv_trans V (P Q R : StateAssertion V) :
+  P <<->> Q ->
+  Q <<->> R ->
+  P <<->> R.
+Proof.
+  repeat rewrite equiv_sa_equiv. intros. etransitivity; eauto.
+Qed.
+
+Lemma length_n_new_cells V l n :
+  List.length (@n_new_cells_from V l n) = n.
+Proof.
+  destruct l as [k]. revert k. induction n; simpl; auto.
+Qed.
+
+Lemma NoDup_insert A (x : A) (l1 l2 : list A) :
+  ~ List.In x (l1 ++ l2) ->
+  List.NoDup (l1 ++ l2) ->
+  List.NoDup (l1 ++ x::l2).
+Proof.
+  induction l1; simpl; intros Hnin Hnodup.
+  - auto using List.NoDup.
+  - inversion Hnodup. unfold not in *. constructor.
+    + unfold not. intros [-> | Hin]%List.in_elt_inv; auto.
+    + auto.
+Qed.
+
+Lemma array_content_label_le V A n n' c m :
+  @array_content V A (Lab (OfNat n)) c m ->
+  List.In (OfNat n') (labels m) ->
+  n <= n'.
+Proof.
+  unfold labels. intros Harray. remember (Lab (OfNat n)) as l eqn:Hl.
+  generalize dependent n. induction Harray; simpl.
+  - contradiction.
+  - intros ? [=->] **.
+    match goal with
+    | [Hinter : Interweave [_] _ _, Hin : List.In _ _ |- _ ] =>
+      apply Interweave_single_l in Hinter as (?&?&->&->);
+      simpl in *; rewrite List.map_app in Hin; simpl in Hin;
+      apply List.in_elt_inv in Hin as [[=->] | Hin']
+    end.
+    + constructor.
+    + rewrite <- List.map_app in Hin'. apply Le.le_Sn_le_stt.
+      apply IHHarray; auto.
+Qed.
+
+Lemma valid_array_content V A v c m :
+  @array_content V A v c m -> Is_Valid_Map m.
+Proof.
+  unfold Is_Valid_Map, labels. intros Harray. induction Harray; simpl.
+  - constructor.
+  - match goal with
+    | [H : Interweave [_] _ _ |- _ ] =>
+      apply Interweave_single_l in H as (?&?&->&->)
+    end.
+    rewrite List.map_app in *. simpl. apply NoDup_insert; auto. intros Hin.
+    eapply Nat.nle_succ_diag_l. eapply array_content_label_le; [eassumption|].
+    unfold labels. rewrite List.map_app. assumption.
+Qed.
+
+Lemma array_decl_empty_content V n l c m :
+  <(l :\ n \= )> c m -> @array_content V (List.repeat None n) (Lab l) c m.
+Proof.
+  unfold sa_array_decl.
+  destruct l as [nl]. intros (->&->). revert nl.
+  induction n; intros; simpl; econstructor; auto.
+  constructor. apply Interweave_nil_l.
+Qed.
+
+Lemma array_content_nil V v c m :
+  @array_content V nil v c m <-> (<exists> l, <[v = Lab l]>) c m.
+Proof.
+  unfold sa_exists, sa_pure, sa_empty.
+  split.
+  - intros Harray. inversion Harray. eauto.
+  - intros (?&->&->&->). constructor.
+Qed.
+(*
+Corollary array_content_nil_r V v c m :
+  @array_content V nil v c m -> (<exists> l, <[v = Lab l]>) c m.
+Proof.
+  apply array_content_nil.
+Qed.
+*)
+Lemma array_content_cons V x A v c m :
+  @array_content V (x::A) v c m <->
+    (<exists> n, <[v = Lab (OfNat n)]> <*> <(OfNat n :?= x)> <*>
+     array_content A (Lab (OfNat (S n)))) c m.
+Proof.
+  unfold sa_exists, sa_single_any, sa_star, sa_pure, sa_empty.
+  split.
+  - intros Harray. inversion Harray. subst. do 5 eexists.
+    repeat split; eauto 15 using disjoint_maps_nil_l, Interweave_nil_l.
+    unfold disjoint_maps. simpl.
+    eintros ? [<-|[]] ?%array_content_label_le; eauto. lia.
+  - intros
+      (?&?&?&?&?&
+        (?&?&?&?&(->&->&->)&(->&->)&->&?&<-%Interweave_nil_l_inv)&
+        ?&->&?&?).
+    simpl. econstructor; eauto.
+Qed.
+(*
+Lemma array_content_cons_r V x A v c m :
+  @array_content V (x::A) v c m ->
+  (<exists> n, <[v = Lab (OfNat n)]> <*> <(OfNat n :?= x)> <*>
+    array_content A (Lab (OfNat (S n)))) c m.
+Proof.
+  apply array_content_cons.
+Qed.
+*)
+
+Lemma array_content_app V A A' n c m :
+  @array_content V (A ++ A') (Lab (OfNat n)) c m <->
+    (array_content A (Lab (OfNat n)) <*>
+     array_content A' (Lab (OfNat (n + List.length A)))) c m.
+Proof.
+  revert n c m. induction A; intros n; simpl.
+  - rewrite Nat.add_0_r. apply equiv_sa_equiv. eapply sa_equiv_trans.
+    + apply sa_equiv_symm, empty_star_l.
+    + apply star_equiv_l, sa_equiv_symm.
+      eapply sa_equiv_trans; apply equiv_sa_equiv.
+      * apply array_content_nil.
+      * unfold sa_empty. split.
+        -- intros. normalize_star. subst. auto.
+        -- intros (->&->). solve_star. rewrite pure_spec. eauto.
+  - rewrite Nat.add_succ_r. intros. rewrite array_content_cons.
+    apply equiv_sa_equiv. eapply sa_equiv_symm, sa_equiv_trans.
+    + eapply star_equiv_l, equiv_sa_equiv, array_content_cons.
+    + eapply sa_equiv_trans.
+      * apply star_exists_equiv_l.
+      * apply sa_exists_equiv. intros. eapply sa_equiv_trans.
+        -- apply sa_equiv_symm, star_assoc.
+        -- eapply sa_equiv_symm, sa_equiv_trans.
+          ++ apply star_equiv_r, equiv_sa_equiv. intros. apply IHA.
+          ++ simpl. apply equiv_sa_equiv. intros.
+            split; intros; normalize_star;
+            match goal with
+            | [H : ?f _ = ?f _ |- _] => injection H as ->
+            end;
+            solve_star.
+Qed.
+
+Fact single_single_any (V : Set) l (v : Value V) :
+  sa_single l v <<->> sa_single_any l (Some v).
+Proof.
+  unfold_all. auto.
+Qed.
+
+Fact single_single_any_l (V : Set) l (v : Value V) :
+  sa_single_any l (Some v) ->> sa_single l v.
+Proof.
+  apply single_single_any.
+Qed.
+
+Fact single_single_any_r (V : Set) l (v : Value V) :
+  sa_single l v ->> sa_single_any l (Some v).
+Proof.
+  apply single_single_any.
 Qed.
 
 Ltac solve_simple_triple n :=
@@ -387,6 +828,16 @@ Theorem triple_value' (V : Set) (v : Value V) (P : StateAssertion V) :
   triple v P (fun v' => <[v' = v]> <*> P).
 Proof.
   solve_simple_triple_30.
+Qed.
+
+Theorem triple_value_implies (V : Set) (v : Value V) (P : StateAssertion V) Q :
+  P ->> Q v ->
+  triple v P Q.
+Proof.
+  intros H. eapply triple_weaken, triple_frame, triple_value.
+  - apply empty_star_l_intro.
+  - apply implies_post_spec. intros. normalize_star. subst. apply H.
+    assumption.
 Qed.
 
 Theorem htriple_value_untimed (V : Set) (v : Value V) (P : StateAssertion V) :
@@ -449,21 +900,6 @@ Proof.
   inversion_cost_red. inversion_red.
 *)
 
-Ltac normalize_star :=
-  repeat match goal with
-  | [H : ((_ <*> _) <*> _) ?c ?m |- _] => apply star_assoc_r in H
-  | [H : (<[_]> <*> _) ?c ?m |- _] => apply star_pure_l in H as [? ?]
-  | [H : ((<exists> _, _) <*> _) ?c ?m |- _] => apply star_exists_l in H as [? ?]
-  | [H : (<exists> _, _) ?c ?m |- _] => destruct H
-  end.
-
-Ltac solve_star :=
-  repeat match goal with
-  | [|- ((_ <*> _) <*> _) ?c ?m ] => apply star_assoc_l; eauto
-  | [|- (<[_]> <*> _) ?c ?m ] => apply star_pure_l; split; auto
-  | [|- ((<exists> _, _) <*> _) ?c ?m ] => apply star_exists_l; eexists; eauto
-  | [|- (<exists> _, _) ?c ?m] => eexists
-  end.
 (*
 Ltac solve_assertion :=
   repeat match goal with
@@ -1128,12 +1564,122 @@ Proof.
   solve_triple_15 big_red_get.
 Qed.
 
+Lemma valid_map_Interweave (V : Set) (m1 m2 m3 : Map V) :
+  Is_Valid_Map m1 ->
+  Is_Valid_Map m2 ->
+  disjoint_maps m1 m2 ->
+  Interweave m1 m2 m3 ->
+  Is_Valid_Map m3.
+Proof.
+  unfold Is_Valid_Map, disjoint_maps, labels.
+  intros Hvalid1 Hvalid2 Hdisjoint Hinter.
+  induction Hinter; simpl in *; constructor;
+    match goal with
+    | [H : List.NoDup (_ :: _) |- _] => inversion H
+    end;
+    eauto; intro; unfold not in *;
+    match goal with
+    | [Hin : List.In (?g _) _ |- _] =>
+      eapply in_Interweave_or in Hin as [? | ?];
+      try (apply map_Interweave with (f := g); eassumption)
+    end;
+    eauto.
+Qed.
+
+Lemma valid_map_app (V : Set) (m1 m2 : Map V) :
+  Is_Valid_Map m1 ->
+  Is_Valid_Map m2 ->
+  disjoint_maps m1 m2 ->
+  Is_Valid_Map (m1 ++ m2)%list.
+Proof.
+  eauto using valid_map_Interweave, Interweave_app.
+Qed.
+
+Lemma n_new_cells_from_mono (V : Set) n k n' :
+  List.In (OfNat n') (labels (n_new_cells_from (V := V) (OfNat n) k)) ->
+  n <= n'.
+Proof.
+  unfold labels. revert n. induction k; intros n []; subst; simpl in *.
+  - injection H. lia.
+  - eauto using le_S_n, le_S, IHk.
+Qed.
+
+Lemma valid_n_new_cells_from (V : Set) l k :
+  Is_Valid_Map (n_new_cells_from (V := V) l k).
+Proof.
+  unfold Is_Valid_Map. destruct l as [n]. revert n.
+  induction k; simpl; constructor; auto.
+  intros Hin. apply n_new_cells_from_mono in Hin. lia.
+Qed.
+
+Lemma disjoint_maps_n_new_cells_from (V : Set) n (m : Map V) :
+  disjoint_maps (n_new_cells_from (new_label m) n) m.
+Proof.
+  unfold disjoint_maps, new_label. intros [n'] Hin_new Hin_m1.
+  apply n_new_cells_from_mono in Hin_new. pose proof max_list_max.
+  eapply List.Forall_forall in H; eauto using (List.in_map of_label).
+  simpl in *. lia.
+Qed.
+
+Lemma valid_map_alloc_array (V : Set) n l (m1 m2 : Map V) :
+  Is_Valid_Map m1 ->
+  (m2,l) = alloc_array n m1 ->
+  Is_Valid_Map m2.
+Proof.
+  unfold alloc_array. intros Hvalid Halloc. injection Halloc as -> _.
+  apply valid_map_app;
+    auto using valid_n_new_cells_from, disjoint_maps_n_new_cells_from.
+Qed.
+
+Lemma labels_Assignment (V : Set) l v (m1 m2 : Map V) :
+  Assignment l v m1 m2 ->
+  labels m1 = labels m2.
+Proof.
+  unfold labels. intros Hassign. induction Hassign; simpl; f_equal.
+  assumption.
+Qed.
+
+Lemma valid_map_Assignment_is_valid (V : Set) l v (m1 m2 : Map V) :
+  Is_Valid_Map m1 ->
+  Assignment l v m1 m2 ->
+  Is_Valid_Map m2.
+Proof.
+  unfold Is_Valid_Map. intros Hvalid Hassign.
+  erewrite <- labels_Assignment; eauto.
+Qed.
+
+Lemma labels_Dealloc (V : Set) l (m1 m2 : Map V) :
+  Dealloc l m1 m2 ->
+  List.incl (labels m2) (labels m1).
+Proof.
+  unfold List.incl, labels. intros Hdealloc.
+  induction Hdealloc; simpl; intros l' Hin; auto. destruct Hin; auto.
+Qed.
+
+Lemma valid_map_Dealloc (V : Set) l (m1 m2 : Map V) :
+  Is_Valid_Map m1 ->
+  Dealloc l m1 m2 ->
+  Is_Valid_Map m2.
+Proof.
+  unfold Is_Valid_Map. intros Hvalid Hdealloc.
+  induction Hdealloc; simpl in *; inversion Hvalid; auto.
+  constructor; auto. unfold not in *. pose proof labels_Dealloc.
+  unfold List.incl in *. eauto.
+Qed.
+
 Lemma valid_map_cost_red (V : Set) e (v : Value V) m1 m2 c :
   Is_Valid_Map m1 ->
   C[e,m1 ~~> v,m2|c] ->
   Is_Valid_Map m2.
 Proof.
-  intros Hvalid Hred. eapply uniqueness_full in Hvalid as (?&?&?&?); eauto.
+  intros Hvalid Hred. induction Hred; auto.
+  apply IHHred. clear Hred IHHred.
+  induction H; subst;
+    eauto 2 using
+      Is_Valid_Map_cons_new,
+      valid_map_alloc_array,
+      valid_map_Assignment_is_valid,
+      valid_map_Dealloc.
 Qed.
 
 Theorem htriple_ref (V : Set) (e : Expr V) P Q :
@@ -1150,7 +1696,7 @@ Proof.
   intros ? [? | []] ?. subst. eauto.
 Qed.
 
-Theorem triple_ref (V : Set) (e : Expr V) (v : Value V) P Q :
+Theorem triple_ref (V : Set) (e : Expr V) P Q :
   triple e P Q ->
   triple (Ref e)
     (sa_credits 1 <*> P)
@@ -1168,14 +1714,82 @@ Proof.
   intros ? [? | []] ?. subst. eauto.
 Qed.
 
+Theorem htriple_new_array (V : Set) (e : Expr V) P Q :
+  hoare_triple e
+    P
+    (fun v => <exists> i, <[v = Int i]> <*> <[(i >= 0)%Z]> <*> Q i) ->
+  hoare_triple (NewArray e)
+    (sa_credits 1 <*> P)
+    (fun v =>
+      <exists> i l, <[v = Lab l]> <*> sa_array_decl l (Z.to_nat i) <*> Q i).
+Proof.
+  unfold hoare_triple. intros. make_cred_positive. edestruct_direct.
+  invert_Intwv_nil. edestruct_all. normalize_star. subst. split_all.
+  - eapply big_red_new_array; eauto. unfold alloc_array. auto.
+  - solve_star. unfold sa_star, sa_array_decl.
+    split_all; eauto using Interweave_app, disjoint_maps_n_new_cells_from.
+  - eapply valid_map_alloc_array in H5; unfold alloc_array; eauto.
+  - assumption.
+Qed.
+
+Theorem htriple_new_array_content (V : Set) (e : Expr V) P Q :
+  hoare_triple e
+    P
+    (fun v => <exists> i, <[v = Int i]> <*> <[(i >= 0)%Z]> <*> Q i) ->
+  hoare_triple (NewArray e)
+    (sa_credits 1 <*> P)
+    (fun v =>
+      <exists> i, array_content (List.repeat None (Z.to_nat i)) v <*> Q i).
+Proof.
+  intros. eapply htriple_weaken, htriple_new_array; eauto using implies_refl.
+  apply implies_post_spec. intros. normalize_star. subst. solve_star.
+  eapply star_implies_mono; try eassumption.
+  { apply implies_spec, array_decl_empty_content. }
+  { apply implies_refl. }
+Qed.
+
+Theorem triple_new_array (V : Set) (e : Expr V) P Q :
+  triple e
+    P
+    (fun v => <exists> i, <[v = Int i]> <*> <[(i >= 0)%Z]> <*> Q i) ->
+  triple (NewArray e)
+    (sa_credits 1 <*> P)
+    (fun v =>
+      <exists> i l, <[v = Lab l]> <*> sa_array_decl l (Z.to_nat i) <*> Q i).
+Proof.
+  unfold triple, hoare_triple. intros. normalize_star. make_cred_positive.
+  edestruct_direct. invert_Intwv_nil. fold_star. edestruct_all. normalize_star.
+  subst. unfold sa_star in H13. edestruct_direct. split_all.
+  - eapply big_red_new_array; eauto. unfold alloc_array. auto.
+  - solve_star. unfold sa_star, sa_array_decl.
+    split_all; eauto using Interweave_app, disjoint_maps_n_new_cells_from.
+  - eapply valid_map_alloc_array in H10; unfold alloc_array; eauto.
+  - lia.
+Qed.
+
+Theorem triple_new_array_content (V : Set) (e : Expr V) P Q :
+  triple e
+    P
+    (fun v => <exists> i, <[v = Int i]> <*> <[(i >= 0)%Z]> <*> Q i) ->
+  triple (NewArray e)
+    (sa_credits 1 <*> P)
+    (fun v =>
+      <exists> i, array_content (List.repeat None (Z.to_nat i)) v <*> Q i).
+Proof.
+  intros. eapply triple_weaken, triple_new_array; eauto using implies_refl.
+  apply implies_post_spec. intros. normalize_star. subst. solve_star.
+  eapply star_implies_mono; try eassumption.
+  { apply implies_spec, array_decl_empty_content. }
+  { apply implies_refl. }
+Qed.
+
 Lemma valid_map_Lookup (V : Set) l v (m : Map V) :
-  Is_Valid_Map m ->
-  List.In (l,v) m ->
+  List.In (l, Some v) m ->
   Lookup l m v.
 Proof.
   unfold Is_Valid_Map. unfold_all. revert l v. induction m; simpl; intros.
   - contradiction.
-  - inversion H. destruct H0 as [-> | ?]; eauto_lr.
+  - destruct H as [-> | ?]; eauto_lr.
 Qed.
 
 Theorem htriple_deref (V : Set) (e : Expr V) (v : Value V) l P Q :
@@ -1184,13 +1798,13 @@ Theorem htriple_deref (V : Set) (e : Expr V) (v : Value V) l P Q :
     (fun v' => <[v' = Lab l]> <*> <(l :== v)> <*> Q) ->
   hoare_triple (Deref e)
     (sa_credits 1 <*> <(l :== v)> <*> P)
-    (fun v => <(l :== v)> <*> Q).
+    (fun v' => <[v' = v']> <*> <(l :== v)> <*> Q).
 Proof.
   unfold hoare_triple. intros. normalize_star. make_cred_positive.
   edestruct_direct. fold_star. repeat invert_Intwv_nil. edestruct_all.
   simpl in *. injection_on_all S. normalize_star. subst.
   split_all; try eapply big_red_deref; simpl in *;
-    eauto using valid_map_Lookup with lamref.
+    eauto using valid_map_Lookup with lamref; solve_star.
   unfold_all_in H10. edestruct_direct.
   eapply valid_map_Lookup, in_or_Interweave; eauto. simpl. auto.
 Qed.
@@ -1206,7 +1820,7 @@ Theorem triple_deref (V : Set) (e : Expr V) (v : Value V) l P Q :
     (fun v' => <[v' = Lab l]> <*> <(l :== v)> <*> Q) ->
   triple (Deref e)
     (sa_credits 1 <*> <(l :== v)> <*> P)
-    (fun v => <(l :== v)> <*> Q).
+    (fun v' => <[v' = v]> <*> <(l :== v)> <*> Q).
 Proof.
   unfold triple, hoare_triple. intros. normalize_star. make_cred_positive.
   edestruct_direct. fold_star. fold_star. conormalize_star.
@@ -1218,14 +1832,41 @@ Proof.
   eapply valid_map_Lookup, in_or_Interweave; eauto. simpl. auto.
 Qed.
 
+Theorem htriple_shift (V : Set) (e1 e2 : Expr V) P Q1 Q2 :
+  hoare_triple e1
+    P
+    (fun v => <exists> n, <[v = Lab (OfNat n)]> <*> Q1 n) ->
+  (forall n, hoare_triple e2
+    (Q1 n)
+    (fun v => <exists> i, <[v = Int i]> <*> <[(i >= 0)%Z]> <*> Q2 n i)) ->
+  hoare_triple (Shift e1 e2)
+    (sa_credits 1 <*> P)
+    (fun v => <exists> n i, <[v = Lab (OfNat (n + Z.to_nat i))]> <*> Q2 n i).
+Proof.
+  solve_htriple_15 big_red_shift.
+Qed.
+
+Theorem triple_shift (V : Set) (e1 e2 : Expr V) P Q1 Q2 :
+  triple e1
+    P
+    (fun v => <exists> n, <[v = Lab (OfNat n)]> <*> Q1 n) ->
+  (forall n, triple e2
+    (Q1 n)
+    (fun v => <exists> i, <[v = Int i]> <*> <[(i >= 0)%Z]> <*> Q2 n i)) ->
+  triple (Shift e1 e2)
+    (sa_credits 1 <*> P)
+    (fun v => <exists> n i, <[v = Lab (OfNat (n + Z.to_nat i))]> <*> Q2 n i).
+Proof.
+  solve_triple_15 big_red_shift.
+Qed.
+
 Lemma valid_map_Assignment (V : Set) l v v' (m : Map V) :
-  Is_Valid_Map m ->
   List.In (l,v) m ->
   Assignment l v' m (update l v' m).
 Proof.
   unfold Is_Valid_Map. unfold_all. revert l v. induction m; simpl; intros.
   - contradiction.
-  - inversion H. destruct l as (n). destruct H0 as [-> | ?].
+  - destruct l as (n). destruct H as [-> | ?].
     + unfold_all_lab. rewrite Nat.eqb_refl. constructor.
     + destruct a as ((n')&?). unfold_all_lab. destruct Nat.eqb_spec with n n'.
       * subst. constructor.
@@ -1283,17 +1924,16 @@ Proof.
       rewrite labels_update; unfold labels; auto.
 Qed.
 
-(* TODO *)
-Theorem htriple_assign (V : Set) (e1 e2 : Expr V) (v v' : Value V) l P1 P2 Q2 :
+Theorem htriple_assign (V : Set) (e1 e2 : Expr V) (v : option (Value V)) l P1 P2 Q2 :
   hoare_triple e1
-    (<(l :== v)> <*> P1)
-    (fun v'' => <[v'' = Lab l]> <*> <(l :== v)> <*> P2) ->
+    (<(l :?= v)> <*> P1)
+    (fun v'' => <[v'' = Lab l]> <*> <(l :?= v)> <*> P2) ->
   hoare_triple e2
-    (<(l :== v)> <*> P2)
-    (fun v'' => <[v'' = v']> <*> <(l :== v)> <*> Q2) ->
+    (<(l :?= v)> <*> P2)
+    (fun v' => <(l :?= v)> <*> Q2 v') ->
   hoare_triple (Assign e1 e2)
-    (sa_credits 1 <*> <(l :== v)> <*> P1)
-    (fun v'' => <[v'' = U_val]> <*> <(l :== v')> <*> Q2).
+    (sa_credits 1 <*> <(l :?= v)> <*> P1)
+    (fun v'' => <[v'' = U_val]> <*> <exists> v', <(l :== v')> <*> Q2 v').
 Proof.
   unfold hoare_triple. intros. normalize_star. make_cred_positive.
   edestruct_direct. fold_star. repeat invert_Intwv_nil.
@@ -1310,16 +1950,16 @@ Proof.
   lia.
 Qed.
 
-Theorem triple_assign (V : Set) (e1 e2 : Expr V) (v v' : Value V) l P1 P2 Q2 :
+Theorem triple_assign (V : Set) (e1 e2 : Expr V) (v : option (Value V)) l P1 P2 Q2 :
   triple e1
-    (<(l :== v)> <*> P1)
-    (fun v'' => <[v'' = Lab l]> <*> <(l :== v)> <*> P2) ->
+    (<(l :?= v)> <*> P1)
+    (fun v'' => <[v'' = Lab l]> <*> <(l :?= v)> <*> P2) ->
   triple e2
-    (<(l :== v)> <*> P2)
-    (fun v'' => <[v'' = v']> <*> <(l :== v)> <*> Q2) ->
+    (<(l :?= v)> <*> P2)
+    (fun v' => <(l :?= v)> <*> Q2 v') ->
   triple (Assign e1 e2)
-    (sa_credits 1 <*> <(l :== v)> <*> P1)
-    (fun v'' => <[v'' = U_val]> <*> <(l :== v')> <*> Q2).
+    (sa_credits 1 <*> <(l :?= v)> <*> P1)
+    (fun v'' => <[v'' = U_val]> <*> <exists> v', <(l :== v')> <*> Q2 v').
 Proof.
   unfold triple, hoare_triple. intros. normalize_star. make_cred_positive.
   edestruct_direct. fold_star. fold_star. repeat invert_Intwv_nil.
@@ -1335,6 +1975,51 @@ Proof.
   { destruct l. unfold_all_lab. rewrite Nat.eqb_refl in H24. eassumption. }
   { unfold not. intros. apply List.in_map with (f := fst) in H26. eauto. } }
   lia.
+Qed.
+
+Lemma dealloc_Interweave (V : Set) l ov (m1 m2 : Map V) :
+  Interweave [(l,ov)]%list m1 m2 ->
+  Dealloc l m2 m1.
+Proof.
+  remember [(l,ov)]%list as m0 eqn:Hm0. intros Hinter. induction Hinter.
+  - discriminate.
+  - injection Hm0 as -> ->. invert_Intwv_nil. constructor.
+  - subst. constructor. auto.
+Qed.
+
+Theorem htriple_free (V : Set) (e : Expr V) l ov P Q :
+  hoare_triple e
+    (sa_single_any l ov <*> P)
+    (fun v => <[v = Lab l]> <*> sa_single_any l ov <*> Q) ->
+  hoare_triple (Free e)
+    (sa_credits 1 <*> sa_single_any l ov <*> P)
+    (fun v => <[v = U_val]> <*> Q).
+Proof.
+  unfold hoare_triple. intros. normalize_star. make_cred_positive.
+  edestruct_direct. invert_Intwv_nil. fold_star. edestruct_all. normalize_star.
+  subst. find_star_and_unfold_all. edestruct_direct.
+  split_all;
+    eauto using big_red_free, Interweave_valid_r, dealloc_Interweave with lamref.
+  - solve_star. eassumption.
+  - lia.
+Qed.
+
+Theorem triple_free (V : Set) (e : Expr V) l ov P Q :
+  triple e
+    (sa_single_any l ov <*> P)
+    (fun v => <[v = Lab l]> <*> sa_single_any l ov <*> Q) ->
+  triple (Free e)
+    (sa_credits 1 <*> sa_single_any l ov <*> P)
+    (fun v => <[v = U_val]> <*> Q).
+Proof.
+  unfold triple, hoare_triple. intros. normalize_star. make_cred_positive.
+  edestruct_direct. invert_Intwv_nil. fold_star. fold_star. conormalize_star.
+  edestruct_all. normalize_star. subst. find_star_and_unfold_all.
+  edestruct_direct. fold_disjoint_maps. fold_disjoint_maps. fold_star_with Q.
+  split_all;
+    eauto using big_red_free, Interweave_valid_r, dealloc_Interweave with lamref.
+  - solve_star. eassumption.
+  - lia.
 Qed.
 
 Theorem htriple_seq (V : Set) (e1 e2 : Expr V) P1 Q1 Q2 :
@@ -1501,75 +2186,340 @@ Proof.
   - lia.
 Qed.
 
-(** facts about StateAssertion *)
+(* other facts *)
 
-Fact credits_star_l (V : Set) c1 c2 c :
-  c = c1 + c2 ->
-  sa_credits c1 <*> sa_credits c2 ->> sa_credits (V := V) c.
+Theorem htriple_fun_app (V : Set) (v : Value V) e P Q1 Q2 :
+  triple_fun v Q1 Q2 ->
+  hoare_triple e P Q1 ->
+  hoare_triple (v <* e) P Q2.
 Proof.
-  unfold_all. intros. edestruct_direct. invert_Intwv_nil. auto.
+  unfold triple_fun. intros.
+  assert (forall v' : Value V, hoare_triple (v <* v') (Q1 v') Q2).
+  { auto using htriple_of_triple. }
+  unfold hoare_triple in *. intros. edestruct_all.
+  split_all; eauto using cost_red_comp, cost_red_app2, big_red_app. lia.
 Qed.
 
-Fact credits_star_r (V : Set) c1 c2 c :
-  c = c1 + c2 ->
-  sa_credits (V := V) c ->> sa_credits c1 <*> sa_credits c2.
+Theorem triple_fun_app (V : Set) (v : Value V) e P Q1 Q2 :
+  triple_fun v Q1 Q2 ->
+  triple e P Q1 ->
+  triple (v <* e) P Q2.
 Proof.
-  unfold_all. intros. edestruct_direct. split_all; auto using Interweave_nil.
+  unfold triple_fun. intros.
+  unfold triple, hoare_triple in *. intros. edestruct_all.
+  split_all; eauto using cost_red_comp, cost_red_app2, big_red_app. lia.
 Qed.
 
-Fact implies_trans (V : Set) (P Q R : StateAssertion V) :
-  P ->> Q ->
-  Q ->> R ->
-  P ->> R.
+Theorem triple_fun_app2 (V : Set) (e1 e2 : Expr V) P1 P2 Q1 Q2 :
+  triple e1 P1 (fun v => <[triple_fun v Q1 Q2]> <*> P2) ->
+  triple e2 P2 Q1 ->
+  triple (e1 <* e2) P1 Q2.
 Proof.
-  unfold_all. auto.
+  unfold triple_fun. intros.
+  unfold triple, hoare_triple in *. intros. edestruct_all. normalize_star.
+  edestruct_all.
+  split_all;
+    eauto using cost_red_comp, cost_red_app1, cost_red_app2, big_red_app.
+  lia.
 Qed.
 
-Fact implies_spec (V : Set) (P Q : StateAssertion V) :
-  (P ->> Q) <-> forall c m, P c m -> Q c m.
+Theorem triple_fun_frame (V : Set) (v : Value V) P Q H :
+  triple_fun v P Q ->
+  triple_fun v (P <*>+ H) (Q <*>+ H).
 Proof.
-  unfold_all. reflexivity.
+  unfold triple_fun. auto using triple_frame.
 Qed.
 
-Fact implies_post_spec (V : Set) (P Q : Value V -> StateAssertion V) :
-  (P -->> Q) <-> forall v c m, P v c m -> Q v c m.
+Theorem triple_fun_weaken (V : Set) (v : Value V) P' P Q Q' :
+  P' -->> P ->
+  Q -->> Q' ->
+  triple_fun v P Q ->
+  triple_fun v P' Q'.
 Proof.
-  unfold_all. reflexivity.
+  unfold triple_fun. eauto using triple_weaken.
 Qed.
 
-Fact empty_star_l_intro (V : Set) (P : StateAssertion V) :
-  P ->> <[]> <*> P.
+Lemma triple_value_inv (V : Set) (v : Value V) P Q c m :
+  triple v P Q ->
+  Is_Valid_Map m ->
+  P c m -> Q v c m.
 Proof.
-  unfold_all. intros. split_all; eauto using Interweave_nil_l.
+  unfold triple, hoare_triple. intros Htriple Hvalid HP.
+  specialize Htriple
+    with <[]> c m
+    as (v'&c'&c2&m'
+      &([=->]&->&->)%cost_red_value
+      &HQ%empty_star_r_cancel
+      &Hvalid'
+      &->);
+    auto.
+  apply empty_star_r_intro. assumption.
 Qed.
 
-Fact empty_star_r_intro (V : Set) (P : StateAssertion V) :
-  P ->> P <*> <[]>.
+(*Lemma triple_app_inv (V : Set) (e e' : Expr V) P Q c m :
+  Is_Valid_Map m ->
+  P c m ->
+  triple (e <* e') P Q ->
+  exists P' Q1,
+    triple e P
+      (fun v => <exists> e1',
+        <[v = (-\e1') /\ forall v, triple (subst_e e1' v) (Q1 v) Q]> <*> P') /\
+    triple e' P' Q1.
 Proof.
-  unfold_all. intros. split_all; eauto using Interweave_nil_r.
+  unfold triple, hoare_triple. intros Hvalid HP Htriple.
+  edestruct Htriple
+    as (?&?&?&?&
+      (?&?&?&?&?&?&?&?&?&?&?)%big_red_app_inv&
+      ?%empty_star_r_cancel&?&?);
+    [|apply empty_star_r_intro|]; try eassumption.
+Admitted.*)
+(*
+Lemma triple_app_values_inv (V : Set) (v : Value V) Q :
+  (forall v' : Value V, triple (v <* v') ($1 <*> <[]>) Q) ->
+  exists e1',
+    v = (-\e1') /\ forall v, triple (subst_e e1' v) <[]> Q.
+Proof.
+  unfold triple, hoare_triple. intros Htriple.
+  destruct (Htriple U_val <[]> 1 [])%list
+    as (?&?&?&?&
+      (?&?&?&?&?&?&?&
+        ([=<-]&->&->)%cost_red_value&
+        ?&?&?)%big_red_app_inv&
+      ?%empty_star_r_cancel&?&?).
+  - unfold Is_Valid_Map, labels. simpl. constructor.
+  - do 2 apply empty_star_r. unfold sa_credits. auto.
+  - eexists. split; eauto. intros. apply empty_star_l_cancel in H7.
+Abort.
+*)
+(*
+Theorem triple_fun_n_ary_app_inv_general (V : Set) n (e : Expr V) es P1 P2 Q1 Q2 :
+  List.length es = n ->
+  triple e P1 (fun v => <[triple_fun_n_ary_inv n v Q1 Q2]> <*> P2) ->
+  triple_list_inv es P2 Q1 ->
+  triple (n_ary_app_inv e es) ($n <*> P1) Q2.
+Proof.
+  unfold triple_fun_n_ary_inv. revert e P1 P2 Q1 Q2 es.
+  induction n; destruct es; try discriminate; simpl in *; intros [= ] Hfun.
+  - intros Himpl. eapply triple_weaken_valid; [| |eassumption].
+    + intros. apply empty_star_l_cancel. assumption.
+    + simpl. intros. normalize_star.
+      match goal with
+      | [H : forall _, _ -> triple _ _ _ |- _] => rename H into Htriple
+      end.
+      specialize (Htriple nil eq_refl). simpl in Htriple.
+      eapply (triple_value_inv _ _ _ _ _ _ Htriple); eauto.
+  - intros (Q'&Htri&Hlist).
+    apply triple_weaken with (P := $1 <*> ($n <*> P1)) (Q := Q2).
+    { eapply implies_trans; [|apply star_assoc]. apply star_implies_mono.
+      - apply credits_star_r. lia.
+      - apply implies_refl. }
+    { intros. apply implies_refl. }
+    eapply triple_app; auto. eapply IHn; eauto.
+    eapply triple_weaken; eauto using implies_refl. intros. simpl.
+    apply implies_spec. intros. normalize_star. solve_star. intros.
+    assert (forall v1 : Value V, triple (n_ary_app_inv v (List.map Val (v1::vs))) (Q1 (v1::vs)) Q2)%list.
+    { intros. apply H. simpl. auto. }
+    simpl in *.
+    specialize (H (U_val::vs)%list). simpl in *.
+Admitted.
+
+(*Lemma triple_Sn_ary_app_inv (V : Set) n (v : Value V) vs P Q :
+  List.length vs = S n ->
+  triple (n_ary_app v (List.map Val vs)) P Q ->
+  exists e, v = -\e (*/\
+    (forall v0 : Value V,
+      triple (subst_e e v0) P
+        (fun v1 : Value V =>
+          <[ forall vs : list (Value V), List.length vs = n ->
+            triple (n_ary_app v1 (List.map Val vs)) (Q1 (?v :: vs)%list) Q2
+          ]> <*> P))*).
+Proof.
+  destruct vs; try discriminate. simpl.
+Qed.*)
+
+Theorem triple_fun_n_ary_app_general (V : Set) n (e : Expr V) es P1 P2 Q1 Q2 :
+  List.length es = n ->
+  triple e P1 (fun v => <[triple_fun_n_ary n v Q1 Q2]> <*> P2) ->
+  triple_list es P2 Q1 ->
+  triple (n_ary_app e es) ($n <*> P1) Q2.
+Proof.
+  unfold triple_fun_n_ary. revert e P1 P2 Q1 es.
+  induction n; destruct es; try discriminate; simpl in *; intros [= ] Hfun.
+  - intros Himpl. eapply triple_weaken_valid; [| |eassumption].
+    + intros. apply empty_star_l_cancel. assumption.
+    + simpl. intros. normalize_star.
+      match goal with
+      | [H : forall _, _ -> triple _ _ _ |- _] => rename H into Htriple
+      end.
+      specialize (Htriple nil eq_refl). simpl in Htriple.
+      eapply (triple_value_inv _ _ _ _ _ _ Htriple); eauto.
+  - intros (Q'&Htri&Hlist).
+    apply triple_weaken with (P := $n <*> ($1 <*> P1)) (Q := Q2).
+    { eapply implies_trans; [|apply star_assoc]. apply star_implies_mono.
+      - apply credits_star_r. lia.
+      - apply implies_refl. }
+    { intros. apply implies_refl. }
+    eapply IHn; auto. eapply triple_app; eauto.
+    eapply triple_weaken; eauto using implies_refl. intros. simpl.
+    apply implies_spec. intros. normalize_star. (*solve_star.*)
 Qed.
 
-Fact empty_star_l_cancel (V : Set) (P : StateAssertion V) :
-  <[]> <*> P ->> P.
+Theorem triple_fun_n_ary_app (V : Set) n (v : Value V) es P Q1 Q2 :
+  List.length es = n ->
+  triple_fun_n_ary n v Q1 Q2 ->
+  triple_list es P Q1 ->
+  triple (n_ary_app v es) P Q2.
 Proof.
-  unfold_all. intros. edestruct_direct. invert_Intwv_nil. auto.
+  unfold triple_fun_n_ary. revert es. induction n; destruct es; try discriminate; simpl in *.
+  - intros [= ] Hfun Himpl. eapply triple_weaken; eauto. intros.
+    apply implies_refl.
+  - intros [= ] Hfun (Q'&Htri&Hlist). apply IHn.
+    + f_equal.
+Qed.
+*)
+
+Fixpoint triple_list_curry {V : Set} (es : list (Expr V)) (P : StateAssertion V) :
+  n_ary_fun_type (List.length es) (Value V) (StateAssertion V) ->
+  (Value V -> n_ary_fun_type (List.length es) (Value V) (StateAssertion V)) ->
+  ((Value V -> StateAssertion V) -> Prop) ->
+    Prop :=
+  match es with
+  | [] => fun Q Qlast f => P ->> $1 <*> Q -> f Qlast
+  | (e::es') => fun Q Qlast f =>
+    forall Qmid x, triple e P (fun v => <[v = x]> <*> Qmid x) ->
+      triple_list_curry es' (Qmid x) (Q x) (Qlast x) f
+  end%list.
+
+Lemma triple_list_curry_weaken_pre (V : Set) (e : Expr V) es
+  (P1 P1' P2 : StateAssertion V) Q1 Q2 :
+  P1 ->> P1' ->
+  triple_list_curry es P2 Q1 Q2 (triple e P1') ->
+  triple_list_curry es P2 Q1 Q2 (triple e P1).
+Proof.
+  revert P2 Q1 Q2. induction es; simpl; intros P2 Q1 Q2.
+  - intros Himpl1 Htriple Himpl2.
+    eapply triple_weaken; eauto using implies_refl.
+  - intros Himpl1 Htriple_list Qmid x Htriple. eapply IHes; auto.
 Qed.
 
-Fact empty_star_r_cancel (V : Set) (P : StateAssertion V) :
-  P <*> <[]> ->> P.
+Theorem triple_fun_n_ary_app_general (V : Set) (e e' : Expr V) es
+  (P1 P2 : StateAssertion V) Q1 Q2 :
+  triple e P1 (fun v => <[triple_fun_n_ary (List.length es) v Q1 Q2]> <*> P2) ->
+  triple_list_curry (e'::es) P2 Q1 Q2
+    (triple (n_ary_app e (e'::es)) ($(List.length es) <*> P1)).
 Proof.
-  unfold_all. intros. edestruct_direct. rewrite Nat.add_0_r.
-  invert_Intwv_nil. auto.
+  revert e e' P1 P2. induction es (*using List.rev_ind*).
+  - simpl. intros. eapply triple_fun_app2; eauto.
+    eapply triple_weaken; [apply empty_star_l_cancel| |];
+      eauto using implies_refl.
+    intros. simpl. apply implies_spec. intros. normalize_star. solve_star.
+    eapply triple_fun_weaken; eauto using implies_refl.
+    intros. simpl.
+    eauto using
+      implies_trans, star_assoc_l, star_implies_mono, implies_refl, star_comm.
+  - intros. hnf. intros. simpl List.length in *.
+    apply triple_list_curry_weaken_pre with
+      (P1' := $(List.length es) <*> ($1 <*> P1)).
+    { eapply implies_trans; [|apply star_assoc].
+      apply star_implies_mono; auto using implies_refl.
+      apply credits_star_r. lia. }
+    apply IHes.
+    eapply triple_weaken, triple_app; [|
+      lazymatch goal with
+      | [|- forall x, ?Q x ->> @?Q' x] => unify Q Q'
+      end
+    | |]; eauto using implies_refl.
+    simpl in H. eapply triple_weaken; eauto using implies_refl.
+    apply implies_post_spec. intros. normalize_star. unfold triple_fun in *.
+    specialize H1 with x x. apply htriple_of_triple in H1. unfold hoare_triple in H1.
+    destruct (H1 1 []%list)
+      as (?&?&?&?&
+        (?&?&?&?&?&?&?&
+          ([=<-]&->&->)%cost_red_value&
+          ([=<-]&->&->)%cost_red_value&
+          Hred&?)%big_red_app_inv&
+        ?&?&?).
+    + unfold Is_Valid_Map, labels. simpl. constructor.
+    + swap_star. solve_star. unfold sa_credits. auto.
+    + assert (x1=1/\x2=0/\x10=0) as (->&->&->) by lia.
+      apply cost_red_0 in Hred as (Hsubst_e&<-); [|reflexivity].
+      normalize_star. solve_star. split; auto. intros. apply triple_frame.
+      apply triple_pure. intros ->. rewrite Hsubst_e.
+      apply triple_value_implies, implies_spec. intros.
+      normalize_star. subst. apply pure_spec. auto.
 Qed.
 
-Fact empty_spec (V : Set) c (m : Map V) :
-  <[]> c m <-> c = 0 /\ m = []%list.
+Theorem triple_fun_n_ary_app (V : Set) (v : Value V) e es
+  (P : StateAssertion V) Q1 Q2 :
+  triple_fun_n_ary (List.length es) v Q1 Q2 ->
+  triple_list_curry (e::es) P Q1 Q2
+    (triple (n_ary_app v (e::es)) ($(List.length es) <*> P)).
 Proof.
-  unfold_all. reflexivity.
+  intros. apply triple_fun_n_ary_app_general.
+  eapply triple_weaken, triple_frame; [|
+    lazymatch goal with
+    | [|- forall x, ?Q x ->> @?Q' x] => unify Q Q'
+    end
+  |]; eauto using empty_star_l_intro, implies_refl.
+  apply triple_value_implies. apply implies_spec. intros. normalize_star. subst.
+  apply pure_spec. auto.
 Qed.
 
-Fact pure_spec (V : Set) P c (m : Map V) :
-  <[P]> c m <-> P /\ c = 0 /\ m = []%list.
+Fixpoint sa_star_n_ary {V} n :
+  n_ary_fun_type n (Value V) (StateAssertion V) ->
+  n_ary_fun_type n (Value V) (StateAssertion V) ->
+  n_ary_fun_type n (Value V) (StateAssertion V) :=
+  match n with
+  | 0 => fun P Q => P <*> Q
+  | S n' => fun P Q => fun x => sa_star_n_ary n' (P x) (Q x)
+  end.
+
+Fixpoint sa_star_n_ary_post {V} n :
+  n_ary_fun_type (S n) (Value V) (StateAssertion V) ->
+  n_ary_fun_type n (Value V) (StateAssertion V) ->
+  n_ary_fun_type (S n) (Value V) (StateAssertion V) :=
+  match n with
+  | 0 => fun P Q => P <*>+ Q
+  | S n' => fun P Q => fun x => sa_star_n_ary_post n' (P x) (Q x)
+  end.
+
+Theorem triple_fun_n_ary_frame (V : Set) (v : Value V) n Q1 Q2 H :
+  triple_fun_n_ary n v Q1 Q2 ->
+  triple_fun_n_ary n v
+    (sa_star_n_ary (S n) Q1 H) (sa_star_n_ary_post (S n) Q2 H).
 Proof.
-  unfold_all. reflexivity.
+  revert v. induction n; simpl.
+  - intros. eapply triple_fun_weaken; intros.
+    { apply star_assoc_l. }
+    { apply implies_refl. }
+    auto using triple_fun_frame.
+  - intros. simpl in IHn. eapply triple_fun_weaken; auto.
+    { intros. apply implies_refl. }
+    { apply implies_post_spec. intros. normalize_star. subst.
+      apply pure_spec. auto. }
+Qed.
+
+Fixpoint sa_implies_n_ary {V} n :
+  n_ary_fun_type n (Value V) (StateAssertion V) ->
+  n_ary_fun_type n (Value V) (StateAssertion V) ->
+    Prop :=
+  match n with
+  | 0 => fun P Q => P ->> Q
+  | S n' => fun P Q => forall x, sa_implies_n_ary n' (P x) (Q x)
+  end.
+
+Theorem triple_fun_n_ary_weaken (V : Set) (v : Value V) n Q1' Q1 Q2 Q2' :
+  sa_implies_n_ary (S n) Q1' Q1 ->
+  sa_implies_n_ary (S (S n)) Q2 Q2' ->
+  triple_fun_n_ary n v Q1 Q2 ->
+  triple_fun_n_ary n v Q1' Q2'.
+Proof.
+  revert v Q1 Q2. induction n; simpl.
+  - intros. eapply triple_fun_weaken; intros; auto. apply star_implies_mono.
+    { apply implies_refl. }
+    { auto. }
+  - intros. simpl in IHn. eapply triple_fun_weaken; auto.
+    { intros. simpl. apply implies_refl. }
+    { apply implies_post_spec. intros. normalize_star. subst.
+      apply pure_spec. eauto. }
 Qed.
